\subsection{Week 2 (Jan 8--Jan 14)}

\dayentry{2026-01-08}{Rings}
\begin{theorem} 
	Let $f:R \to S$ be a homomorphism of rings, Then 
	\begin{align*}
		&\text{(1)}\quad f(0_R) = 0_S \\
		&\text{(2)}\quad f(-a) = -f(a) \quad \forall a \in R \\
		&\text{(3)}\quad f(a - b) = f(a) - f(b) \quad \forall a,b \in R
	\end{align*}
\end{theorem} 
\begin{proof} 
	(1) As $f$ is a homomorphism of rings, we have the following: 
	\begin{align*} 
		f(0_R) + f(0_R) &= f(0_R + 0_R) \\
		f(0_R) + f(0_R) &= f(0_R) \quad [0_R + 0_R = 0_R \,\text{in} \, R] \\
		f(0_R) + f(0_R) & = f(0_R) + 0_S \, [f(0_R) + 0_S = f(0_R)\, \text{in} \, S] \\
		f(0_R) &= 0_S
	\end{align*} 

	(2) Note that: $f(a) + f(-a) = f(a + (-a)) = f(0_R) = 0_S$ by (1) and $f$ is a homomorphism. So, $f(-a)$ is a solution to the equation $f(a) + x = 0_S$. But as $S$ is a ring, there exists only one unique solution to this equation which is $-f(a)$. Therefore by [theorem to be proved at a later date], $f(-a) = -f(a)$. 

	(3) As $f$ is a homomorphism and by (2), we have the following: 
	\begin{align*}
		f(a - b) &= f(a + (-b)) \\
		&= f(a) + f(-b) \\
		&= f(a) - f(b) 
	\end{align*} 
\end{proof}

\dayentry{2026-01-09}{Rings}
\begin{theorem} 
	Let $f: R \to S$ be a homomorphism of rings. If $R$ is a ring with identity and $f$ is surjective, then 
	\begin{align*}
		&\text{(1)}\quad S \, \text{is a ring with identity}\, f(1_R). \\
		&\text{(2)}\quad \text{Whenever }  u \, \text{is a unit in} \, R, \, \text{then} \, f(u) \, \text{is a unit in} \, S \, \text{and} \, f(u)^{-1} = f(u^{-1}).  
	\end{align*}
\end{theorem}
\begin{proof} 
	(1) Let $s$ be some element in $S$. As $f$ is surjective, there exists some $r \in R$ such that $f(r) = s$. Then we have that 
	\begin{align*}
		s * f(1_R) = f(r)f(1_R) = f(r * 1_R) = f(r) = s
	\end{align*}
	Similarly $f(1_R) * s = s$. Therefore $1_S = f(1_R)$.

	(2) As $u$ is a unit, there exists some $v \in R$ such that $uv = 1_R = vu$. By (1), we have that $f(u)f(v) = f(uv) = f(1_R) = 1_S$. Similarly, $vu = 1_R$ which implies that $f(v)f(u) = 1_S$. Therefore $f(u)$ is a unit in $S$ with inverse $f(v)$. Said differently $f(u)^{-1} = f(v)$. As $v$ is the inverse of $u$ ($v = u^{-1}$), we see that $f(u)^{-1} = f(v) = f(u^{-1})$. 
\end{proof} 
